\documentclass[12pt, leqno]{book}
\usepackage{amsmath,amscd,amsthm,amssymb,amsxtra,latexsym,epsfig,epic,graphics}
\usepackage[matrix,arrow,curve]{xy}
\usepackage{graphicx}
\usepackage{diagrams}
%\usepackage{amsrefs}
%%%%%%%%%%%%%%%%%%%%%%%%%%%%%%%%%%%%%%%%%
%\textwidth16cm
%\textheight20cm
%\topmargin-2cm
\oddsidemargin.8cm
\evensidemargin1cm

%%%%%Definitions
\input preamble.tex
\def\TU{{\bf U}}
\def\AA{{\mathbb A}}
\def\BB{{\mathbb B}}
\def\CC{{\mathbb C}}
\def\QQ{{\mathbb Q}}
\def\RR{{\mathbb R}}
\def\facet{{\bf facet}}
\def\image{{\rm image}}
\def\cE{{\cal E}}
\def\cF{{\cal F}}
\def\cG{{\cal G}}
\def\cH{{\cal H}}
\def\cHom{{{\cal H}om}}
\def\h{{\rm h}}
 \def\bs{{Boij-S\"oderberg{} }}

\makeatletter
\def\Ddots{\mathinner{\mkern1mu\raise\p@
\vbox{\kern7\p@\hbox{.}}\mkern2mu
\raise4\p@\hbox{.}\mkern2mu\raise7\p@\hbox{.}\mkern1mu}}
\makeatother

%%
%\pagestyle{myheadings}
\date{April 30, 2018}
%\date{}
\title{Curves}
%{\normalsize ***Preliminary Version***}} 
\author{David Eisenbud and Joe Harris }

\begin{document}

\chapter{Background}
\section*{Outline}
 Background (corresponds to material in Hartshorne Ch 4, sects 1,2,4(?)---all except elliptic curves and ``classification")
\begin{enumerate}

\item Lasker's Theorem (complete intersections are unmixed) -- sometimes incorrectly called ``$AF+BG$''
state ci implies unmixed; prove by $H^1$ of line bundle.

\item B\'ezout and the  weak B\'ezout (ex 8.4.6 in Fulton).
B\'ezout via Koszul complex, at least in codim 2.

\item Families. Define families. discuss "good and bad" families. example: symmetric product. example: plane curves of degree d. family of line bundles on a curve (or a family of curves.)


\end{enumerate}

\section{The Lasker-Noether Theorem}

A key element in the algebraic study of plane curves initiated by Brill and Noether following Riemann's discoveries was what Noether named the ``Fundamental Lemma on Holomorphic Functions.'' In the original language it said that if the homogeneous forms $F(x_{0},x_{1},x_{2})=0$ and $G(x_{0},x_{1},x_{2})=0$ are the equations of two curves in $\PP^{2}$ that have no component in common, then any form $H$ that locally represents a function (the ``holomorphic functions'' of the name) vanishing on all the points
of the intersection must have an expression $H = AF+BG$, where $A,B$ are also homogeneous forms. It was extended by Lasker to the case of many polynomials (homogeneous or not) in many variables. (This is sometimes called the ``$AF+BG$ Theorem''.) 

\begin{theorem}\label{Lasker}
Suppose that $I = (f_{1}, \dots, f_{c}) \subset \CC[x_{0},\dots,x_{n}]$ is an ideal generated by $c$ homogeneous forms in a polynomial ring. 
If $X:= V(I)$ has codimension $c$, then $I$ is saturated and $\HH^{i}(\cO_{X}(d)) = 0$ for all $0<i<\dim X$ and all $d\in \ZZ$; and if $\dim X\geq 1$
then the map
$\HH^{0}\cO_{\PP^{n}}(d) \to \HH^{0}(\cO_{X}(d)$ is surjective for every $d$.
\end{theorem}

In modern language, the hypothesis says that $f_{1}, \dots, f_{c}$ is a \emph{regular sequence} and $V(f_{1},\dots,f_{c})$ form a \emph{complete intersection}, while the concludsion says that the ring $S/I$ is Cohen-Macaulay. See for example \cite[Chapter 18]{Eisenbud95}, where the result it proven in this generality and more.
We will prove it here only for $c\leq 2$.

Theorem~\ref{Lasker} immediately implies the orginal version of the theorem because (by the Nullstellensatz) the set of forms vanishing on $V(f_{1}, \dots, f_{c})$ is the saturation 
of the ideal $(f_{1}, \dots, f_{c})$. 

\begin{proof} The vanishing in the case $c=0$ is the usual computation of the cohomology of line bundles on $\PP^{n}$.

Write $e_{i}$ for the degree of $f_{i}$. If $c = 1$ then, since the polynomial ring is a domain, we have a short exact sequence
$$
0\to \cO_{\PP^{n}}(-e_{1}) \rTo^{f_{1}}  \cO_{\PP^{n}} \to  \cO_{X}\to 0.
$$
We tensor this sequence with $\cO_{\PP^{n}}(d)$, and pass to cohomology, obtaining a long exact sequence that begins
\begin{align*}
0\to &\HH^{0}(\cO_{\PP^{n}}(d-e_{1})) \rTo^{f_{1}}  \HH^{0}(\cO_{\PP^{n}}(d)) \to  \HH^{0}(\cO_{X}(d))\to\\
&\HH^{1}(\cO_{\PP^{n}}(d-e_{1}))\to \cdots .
\end{align*}
We may break this into two exact sequences
$$
0\to \HH^{0}(\cO_{\PP^{n}}(d-e_{1})) \rTo^{f_{1}}  \HH^{0}(\cO_{\PP^{n}}(d)) \to \cI_{X}(d) \to 0
$$
and 
$$
0 \to \cI_{X}(d) \to \HH^{0}(\cO_{X}(d))\to\HH^{1}(\cO_{\PP^{n}}(d-e_{1}))\to \cdots .
$$ 
The direct sum of the spaces $\HH^{0}(\cO_{\PP^{n}}(d))$ is the polynomial ring, so the exactness of the first sequence shows that $f_{1}$ generates the homogeneous ideal of $X$. If $\dim X\geq 1$ then $n>1$ so the right hand term in the second  vanishes,
proving the last assertion of the Theorem.

Finally, suppose that $c=2$. Since $X$ has codimension 2 the hypersurfaces $f_{1}=0$ and $f_{2}=0$ have no common component---that is, $f_{1}$ and $f_{2}$ are relatively prime. Since the polynomial ring has unique factorization, this implies that the intersection of the ideals $(f_{1})$ and $(f_{2})$ is the ideal
$(f_{1}f_{2})$, or in other words that the natural complex
$$
0\to\cO_{\PP^{n}}(-e_{1}-e_{2}) \rTo^{
\begin{pmatrix}
 f_{2}\\-f_{1}
\end{pmatrix}}
 \cO_{\PP^{n}}(-e_{1})\oplus \cO_{\PP^{n}}(-e_{2}) \rTo^{
 \begin{pmatrix}
 f_{1}&f_{2}
\end{pmatrix}}
\cO_{\PP^{n}}
\to
\cO_{X}
\to 0
$$
is exact. As before, we tensor with $\cO_{\PP^{n}}(d)$ and break the result into the two exact sequences
$$
0\to\cO_{\PP^{n}}(-e_{1}-e_{2}) \rTo^{
\begin{pmatrix}
 f_{2}\\-f_{1}
\end{pmatrix}}
 \cO_{\PP^{n}}(-e_{1})\oplus \cO_{\PP^{n}}(-e_{2}) \rTo^{
 \begin{pmatrix}
 f_{1}&f_{2}
\end{pmatrix}}
\to \cI_{X}(d) \to 0
$$
and
$$
0\to \cI_{X}(d) \to \cO_{\PP^{n}}(d) \to \cO_{X}(d) \to 0.
$$
Taking cohomology we get:
\begin{align*}
0\to\HH^{0}(\cO_{\PP^{n}}(d-e_{1}-e_{2}))
&\rTo^{
\begin{pmatrix}
 f_{2}\\-f_{1}
\end{pmatrix}}
\HH^{0}( \cO_{\PP^{n}}(d-e_{1})\oplus \cO_{\PP^{n}}(d-e_{2}))\\
 &\rTo^{
 \begin{pmatrix}
 f_{1}&f_{2}
\end{pmatrix}}
\HH^{0}(\cI_{X}(d))\to \HH^{1}(\cO_{X}(d-e_{1}-e_{2})) \to \cdots
\end{align*}
and
\begin{align*}
0\to \HH^{0}(\cI_{X}(d))\to
\HH^{0}(\cO_{\PP^{n}}(d))
\to \HH^{0}(\cO_{X}(d)) \to
\HH^{1}(\cI_{X}(d))\to\cdots
\end{align*}
As above, 
\end{proof}
\end{document}